fix cv

cv_translator/backend_64_cvScript.sml
@@ -154,12 +154,29 @@ val _ = stack_allocTheory.compile_def |> arch_spec |> SRULE [stack_allocTheory.s
                                                    |> cv_auto_trans;
 
 val _ = stack_rawcallTheory.seq_stack_alloc_def |> arch_spec |> cv_trans;
-val _ = stack_rawcallTheory.collect_info_def |> arch_spec |> cv_trans;
+val _ = stack_rawcallTheory.add_info_def |> arch_spec |> cv_trans;
+
+Definition collect_info'_def:
+  (collect_info' [] f = f) ∧
+  (collect_info' (x::xs) f =
+    collect_info' xs (add_info f x))
+End
+
+Theorem collect_info'_thm[cv_inline]:
+  ∀ls f.
+  collect_info ls f = collect_info' ls f
+Proof
+  Induct>>
+  rw[collect_info'_def]>>
+  fs[stack_rawcallTheory.collect_info_def]
+QED
+
 val _ = stack_rawcallTheory.dest_case_def |> arch_spec |> cv_trans;
 val _ = stack_rawcallTheory.comp_seq_def |> arch_spec |> cv_trans;
 val _ = stack_rawcallTheory.comp_def |> arch_spec |> cv_trans;
 val _ = stack_rawcallTheory.comp_top_def |> arch_spec |> cv_trans;
 val _ = stack_rawcallTheory.compile_def |> arch_spec |> cv_auto_trans;
+
 val _ = stack_to_labTheory.compile_def |> arch_spec |> cv_auto_trans;
 val _ = word_to_stackTheory.format_var_def |> cv_trans;
 val _ = word_to_stackTheory.wReg1_def |> arch_spec |> cv_trans;
